several comments in many files

src/SimpleTypes.v
@@ -1,3 +1,8 @@
+(** * The simple types
+      This file contains the defintion of simple types [ty] and 
+      some auxiliary definitions.
+    *)
+
 Set Implicit Arguments.
 
 Require Import Arith.Arith_base List Omega.
@@ -35,19 +40,4 @@ Definition eq_ty_dec : forall (t t' : ty), {t = t'} + {t <> t'}.
   pose eq_id_dec.
   decide equality.
 Defined.
-
-(** * Creates a list of type from a list of ids *)
-Fixpoint ty_from_id_list (l : list id) : list ty :=
-  match l with
-  | nil => nil
-  | x::l' => var x :: ty_from_id_list l'
-  end.
-
-Lemma length_ty_from_id_list : forall l : list id, length (ty_from_id_list l) = length l.
-Proof.
-  induction l; simpl; auto.
-Qed.
-
-Hint Resolve length_ty_from_id_list.
-Hint Rewrite length_ty_from_id_list:RE.
 
